

# Quiz 3/12 Answers

COGS 526

1. Translate to first-order logic:

- **[2pts\*]** “Not everything that is faced can be changed, but nothing can be changed until it is faced.” (James Baldwin)

**Predicates:**

- $F(x)$ :  $x$  is faced.
- $C(x)$ :  $x$  can be changed.

“Not everything that is faced can be changed” can be formulated as:

$$\neg(\forall x.F(x) \rightarrow C(x))$$

“Nothing can be changed until it is faced” can be formulated as:

$$\neg(\exists x.\neg F(x) \wedge C(x))$$

The whole formula is the conjunction of two:

$$\begin{aligned} &\neg(\forall x.F(x) \rightarrow C(x)) \wedge \neg(\exists x.\neg F(x) \wedge C(x)) \\ &\equiv \exists x(F(x) \wedge \neg C(x)) \wedge \forall x(C(x) \rightarrow F(x)) \end{aligned}$$

- **[5pts]** “Some cause happiness wherever they go; others whenever they go.” Key:  $R(x)$  : ‘ $x$  is a person’,  $P(x)$  : ‘ $x$  is a place’,  $T(x)$  : ‘ $x$  is a time’,  $C(x, y)$  : ‘ $x$  causes happiness at the place  $y$ ’,  $G(x, y, z)$  : ‘ $x$  goes to place  $y$  at time  $z$ ’,  $L(x, y, z)$  : ‘ $x$  leaves the place  $y$  at time  $z$ ’.

“Some cause happiness wherever they go” can be reformulated as: There exists a person  $x$  such that for all places  $y$  and all times  $z$ , if  $x$  goes to  $y$  at time  $z$ , then  $x$  causes happiness at  $y$ .

$$\exists x.(R(x) \wedge \forall y\forall z.((P(y) \wedge T(z) \wedge G(x, y, z)) \rightarrow C(x, y)))$$

“Others whenever they go” can be reformulated as: There exists a person  $a$  such that for all places  $y$  and all times  $z$ , if  $a$  leaves place  $y$  at time  $z$ , then  $a$  causes happiness at  $y$ .

$$\exists a.(R(a) \wedge \forall y\forall z.((P(y) \wedge T(z) \wedge L(a, y, z)) \rightarrow C(a, y)))$$

The whole expression can be formulated as:

$$\begin{aligned} &\exists x\exists a \left( R(x) \wedge R(a) \wedge x \neq a \right. \\ &\quad \wedge \left[ \forall y\forall z.((P(y) \wedge T(z) \wedge G(x, y, z)) \rightarrow C(x, y)) \right] \\ &\quad \left. \wedge \left[ \forall y\forall z.((P(y) \wedge T(z) \wedge L(a, y, z)) \rightarrow C(a, y)) \right] \right) \end{aligned}$$